WIP: TypingStep Theorem

PiLL/PiLL/Alt.lean
@@ -1,59 +1,112 @@
 import Mathlib.Data.Finset.Basic
 import Mathlib.Tactic
 
-/- Zulip example -/
+-- /- Zulip example -/
+-- abbrev Env := Finset (Nat × Nat)
+-- abbrev HyperEnv := Finset (Env)
+
+-- inductive Typing : HyperEnv → Prop where
+--   | parr {Γ : Env} {x y A B : Nat} :
+--       Typing {Γ ∪ {(y, A)} ∪ {(x, B)}} →
+--       Typing {Γ ∪ {(x, A + B)}}
+
+-- inductive TS1 : HyperEnv → List (Nat × Nat) →
+--   HyperEnv → Prop where
+--   | parr
+--       {Γ : Env} {x y A B : Nat}
+--       (𝒟 : Typing {Γ ∪ {(x, A + B)}})
+--       (𝒟' : Typing {Γ ∪ {(y, A)} ∪ {(x, B)}}) :
+--       TS1
+--         {Γ ∪ {(x, A + B)}}
+--         [(x, y)]
+--         {Γ ∪ {(y, A)} ∪ {(x, B)}}
+
+-- inductive TS2 : ∀ {𝒢 𝒢' : HyperEnv},
+--   Typing 𝒢 → List (Nat × Nat) → Typing 𝒢' → Prop where
+--   | parr
+--       {Γ : Env} {x y A B : Nat}
+--       (𝒟 : Typing {Γ ∪ {(y, A)} ∪ {(x, B)}}) :
+--       TS2
+--         (Typing.parr 𝒟)
+--         [(x, y)]
+--         𝒟
+
+-- theorem swap_last_two (A B C : Env) : A ∪ B ∪ C = A ∪ C ∪ B := by aesop
+-- theorem move_last_two_left (A B C D : Env) : A ∪ B ∪ C ∪ D = A ∪ D ∪ B ∪ C := by aesop
+
+-- theorem example1 {Γ : Env} {x y z A B : Nat}
+--   (𝒟 : Typing {Γ ∪ {(x, A + B)} ∪ {(z, 0)}})
+--   (𝒟' : Typing {Γ ∪ {(y, A)} ∪ {(x, B)} ∪ {(z, 0)}}) :
+--   TS1
+--     {Γ ∪ {(x, A + B)} ∪ {(z, 0)}}
+--     [(x, y)]
+--     {Γ ∪ {(y, A)} ∪ {(x, B)} ∪ {(z, 0)}} := by
+--   rw [move_last_two_left]
+--   rw [swap_last_two]
+--   apply TS1.parr
+--   · rw [← swap_last_two] ; exact 𝒟
+--   · rw [← move_last_two_left] ; exact 𝒟'
+
+-- theorem example2 {Γ : Env} {x y z A B : Nat}
+--   (𝒟 : Typing {Γ ∪ {(x, A + B)} ∪ {(z, 0)}})
+--   (𝒟' : Typing {Γ ∪ {(y, A)} ∪ {(x, B)} ∪ {(z, 0)}}) :
+--   TS2
+--     𝒟
+--     [(x, y)]
+--     𝒟' := by
+--   rw! [swap_last_two]
+--   rw! [move_last_two_left]
+--   apply TS2.parr
+
+
 abbrev Env := Finset (Nat × Nat)
-abbrev HyperEnv := Finset (Env)
+def Env.mk (x y : Nat) : Env := {(x, y)}
 
-inductive Typing : HyperEnv → Prop where
-  | parr {Γ : Env} {x y A B : Nat} :
-      Typing {Γ ∪ {(y, A)} ∪ {(x, B)}} →
-      Typing {Γ ∪ {(x, A + B)}}
+abbrev HyperEnv := Finset Env
+instance : Coe Env HyperEnv := ⟨fun Γ => ({Γ} : HyperEnv)⟩
 
-inductive TS1 : HyperEnv → List (Nat × Nat) →
-  HyperEnv → Prop where
-  | parr
-      {Γ : Env} {x y A B : Nat}
-      (𝒟 : Typing {Γ ∪ {(x, A + B)}})
-      (𝒟' : Typing {Γ ∪ {(y, A)} ∪ {(x, B)}}) :
-      TS1
-        {Γ ∪ {(x, A + B)}}
-        [(x, y)]
-        {Γ ∪ {(y, A)} ∪ {(x, B)}}
+inductive Proc : Type where
+  | one     (x : Nat) (P : Proc)
 
-inductive TS2 : ∀ {𝒢 𝒢' : HyperEnv},
-  Typing 𝒢 → List (Nat × Nat) → Typing 𝒢' → Prop where
-  | parr
-      {Γ : Env} {x y A B : Nat}
-      (𝒟 : Typing {Γ ∪ {(y, A)} ∪ {(x, B)}}) :
-      TS2
-        (Typing.parr 𝒟)
-        [(x, y)]
-        𝒟
+inductive Typing : HyperEnv → Proc → Prop where
+  | one {P : Proc} {x : Nat} :
+      Typing ∅ P →
+      Typing (Env.mk x 1) (Proc.one x P)
 
-theorem swap_last_two (A B C : Env) : A ∪ B ∪ C = A ∪ C ∪ B := by aesop
-theorem move_last_two_left (A B C D : Env) : A ∪ B ∪ C ∪ D = A ∪ D ∪ B ∪ C := by aesop
+inductive Lbl : Type
+  | one (x : Nat)
 
-theorem example1 {Γ : Env} {x y z A B : Nat}
-  (𝒟 : Typing {Γ ∪ {(x, A + B)} ∪ {(z, 0)}})
-  (𝒟' : Typing {Γ ∪ {(y, A)} ∪ {(x, B)} ∪ {(z, 0)}}) :
-  TS1
-    {Γ ∪ {(x, A + B)} ∪ {(z, 0)}}
-    [(x, y)]
-    {Γ ∪ {(y, A)} ∪ {(x, B)} ∪ {(z, 0)}} := by
-  rw [move_last_two_left]
-  rw [swap_last_two]
-  apply TS1.parr
-  · rw [← swap_last_two] ; exact 𝒟
-  · rw [← move_last_two_left] ; exact 𝒟'
+inductive EnvStep : HyperEnv → Lbl → HyperEnv → Prop where
+  | one {x : Nat} :
+      EnvStep (Env.mk x 1) (.one x) ∅
 
-theorem example2 {Γ : Env} {x y z A B : Nat}
-  (𝒟 : Typing {Γ ∪ {(x, A + B)} ∪ {(z, 0)}})
-  (𝒟' : Typing {Γ ∪ {(y, A)} ∪ {(x, B)} ∪ {(z, 0)}}) :
-  TS2
-    𝒟
-    [(x, y)]
-    𝒟' := by
-  rw! [swap_last_two]
-  rw! [move_last_two_left]
-  apply TS2.parr
+inductive ProcStep : Proc → Lbl → Proc → Prop where
+  | one {P : Proc} {x : Nat} :
+      ProcStep (Proc.one x P) (.one x) P
+
+theorem TypingStep {𝒢 ℋ : HyperEnv} {P Q : Proc} {l : Lbl}
+  (hT : Typing 𝒢 P) (hPS : ProcStep P l Q) (hES : EnvStep 𝒢 l ℋ) :
+  Typing ℋ Q := by
+  induction hPS
+  
+  case one P x =>
+    cases hT
+    generalize h𝒢 : (Env.mk x 1 : HyperEnv) = 𝒢 at hES
+    cases hES
+    assumption  
+  
+  -- case one =>
+  --    cases hT
+  --    rename_i 𝒟
+     
+  --    set e := _
+  --    conv at hES =>
+  --      arg 1
+  --      change e
+  --    generalize h : e = e' at hES
+  --    cases hES
+  --    clear! e
+     
+     
+  --    exact 𝒟
+     
